<?xml version="1.0" encoding="UTF-8"?>

<section xml:id="s_cosets_lagrange" xmlns:xi="http://www.w3.org/2001/XInclude">
    <title>Cosets and Lagrange's theorem</title>

    <definition xml:id="d_set_actions">
        <title>Group operations on subsets</title>
        <statement>
            <p>
                Let <m>A</m> be a subset of the group <m>G</m>. Given <m>g\in G</m>, the sets <m>gA</m>, <m>Ag</m>, <m>gAg^{-1}</m> are defined as follows:
                <mdn>
                    <mrow>A^{-1} \amp =\{a^{-1}\mid a\in G\}</mrow>
                    <mrow>gA \amp =\{ga\mid a\in A\}</mrow>
                    <mrow>Ag \amp =\{ag\mid a\in A\}</mrow>
                    <mrow>gAg^{-1} \amp =\{gag^{-1}\mid a\in A \}</mrow>
                </mdn>.
            </p>
        </statement>
    </definition>


    <definition xml:id="d_cosets">
    <title>Coset and coset space</title>
    <statement>
    <p>
    Let <m>H</m> be a subgroup of the group <m>G</m>. Given <m>g\in G</m> the set <m>gH</m> defined 
    as 
    <men xml:id="eq_left_coset">
        gH =\{gh\mid h\in H\}
    </men>
    is called the <term>left <m>H</m>-coset</term> in <m>G</m> corresponding to <m>g</m>, and the set <m>Hg</m> defined as 
    <men xml:id="eq_right_coset">
        Hg=\{hg\mid h\in H\}
    </men>
    is called the <term>right <m>H</m>-coset</term> in <m>G</m> corresponding to <m>g</m>. Elements of a coset are called <term>representatives</term> of that coset. 
    </p>
    <p>
        The set of all left (resp. right) <m>H</m>-cosets is called the <term>left (resp. right) coset space</term> of <m>H</m>, and is denoted <m>G/H</m> (resp. <m>H\backslash G</m>).
    </p>
    </statement>
    </definition>
    <convention>
        <title>Cosets are left cosets by default</title>
        
        <p>
            Unless stated otherwise, a coset in this course will be assumed to be a left coset. 
        </p>
    </convention>
    <example xml:id="eg_cosets_Z">
    <title>Cosets in <m>\Z</m></title>
    <statement>
    <p>
    Recall that any subgroup <m>H</m> of <m>\Z</m> can be described as <m>H=(n)</m> for a unique <m>n\in \Z_{\geq 0}</m>. Show that the cosets of <m>H=(n)</m> are precisely the congruence classes modulo <m>n</m>. 
    </p>
    </statement>
    <solution>
    <p>
    Fix <m>H=(n)</m>.  Given <m>a\in \Z</m> the coset <m>a+H</m> is by definition 
    <md>
        <mrow>a+(n) \amp =\{a+qn\mid q\in \Z\}</mrow>
        <mrow> \amp = [a]_n</mrow>
    </md>.
    This computation shows cosets are congruence classes and vice versa. 
    </p>
    </solution>
    </example>
    <example xml:id="eg_cosets_Zn">
    <title>Cosets in <m>\Z/12\Z</m></title>
    <statement>
    <p>
    Let <m>G=\Z/12\Z</m> and let <m>H=\angvec{\overline{4}}\leq G</m>. Compute <m>G/H</m>. 
    </p>
    </statement>
    <solution>
    <p>
    We have <m>H=\angvec{\overline{4}}=\{0,4,8\}</m>. A simple computation shows 
    <md>
        <mrow>\overline{0}+H \amp = H</mrow>
        <mrow>\overline{1}+H \amp =\{\overline{1},\overline{5},\overline{9}\}</mrow>
        <mrow>\overline{2}+H \amp =\{\overline{2},\overline{6},\overline{10}\}</mrow>
        <mrow>\overline{3}+H \amp = \{\overline{3},\overline{7},\overline{11}\}</mrow>
        <mrow>\overline{4}+H \amp =\{\overline{4},\overline{8},0\}=\{\overline{0},\overline{4},\overline{8}\}=H</mrow>
    </md>.
    This suggests that <m>G/H=\{\overline{0}+H,\overline{1}+H,\overline{2}+H,\overline{3}+H\}</m>. This can be shown by proving that <m>\overline{a}+H=\overline{b}+H</m> if and only if <m>a\equiv b\pmod 4</m>. <xref ref="th_cosets"/> below takes care of this for us. 
    </p>
    </solution>
    </example>
    <example xml:id="eg_cosets_Dn">
    <title>Cosets in <m>D_4</m></title>
    <statement>
    <p>
    Let <m>G=D_4</m> and let <m>H=\angvec{rs}</m>. Compute <m>G/H</m> and <m>H\backslash G</m>. 
    </p>
    </statement>
    <solution>
    <p>
    We have <m>H=\angvec{rs}=\{1, rs\}</m>. We compute
    <md>
        <mrow>1H \amp =H</mrow>
        <mrow>rH= \amp \{r,r^2s\}</mrow>
        <mrow>r^2H \amp =\{r^2, r^3s\}</mrow>
        <mrow>r^3H \amp =\{r^3,s\}</mrow>
        <mrow>sH \amp = \{s,r^3\}=r^3H </mrow>
        <mrow>(rs)H \amp =\{rs, e\}=H</mrow>
        <mrow>(r^2s)H \amp =\{r^2s, r\}=rH</mrow>
        <mrow>(r^3s)H \amp =\{r^3s, r^2\}=r^2H</mrow>
    </md>
    We conclude that <m>G/H=\{H,rH,r^2H,r^3H\}</m>. Let's look at the right cosets: 
    <md>
        <mrow>H1 \amp =H</mrow>
        <mrow>Hr \amp =\{r,s\}</mrow>
        <mrow>Hr^2 \amp =\{r^2,r^3s\}</mrow>
        <mrow>Hr^3 \amp = \{r^3, r^2s\}</mrow>
        <mrow>Hs \amp =\{s,r\}=Hr</mrow>
        <mrow>H(rs) \amp =\{rs, e\}=H</mrow>
        <mrow>H(r^2s) \amp =\{r^2s,r^3\}=Hr^3</mrow>
        <mrow>H(r^3s) \amp =\{r^3s, r^2\}=r^2H</mrow>
    </md>.
    We conclude that <m>H\backslash G=\{H, Hr, Hr^2, Hr^3\}</m>.
    </p>
    </solution>
    </example>
    <theorem xml:id="th_cosets">
    <title>Cosets and coset space</title>
    <statement>
    <p>
    Let <m>H</m> be a subgroup of the group <m>G</m>. 
    <ol>
        <li>
            <p>
                The relation <m>g\sim g'</m> if and only if <m>g'=gh</m> for some <m>h\in H</m> is an equivalence relation and the cosets <m>gH</m> are the corresponding equivalence classes.
            </p>

        </li>
        <li>
            <p>
                Given <m>g,g'\in G</m>, the following statements are equivalent. 
                <ol>
                    <li>
                        <p>
                            <m>gH=g'H</m>.
                        </p>
                    </li>
                    <li>
                        <p>
                            <m>g'\in gH</m>.
                        </p>
                    </li>
                    <li>
                        <p>
                            <m>g^{-1}g'\in H</m>.
                        </p>
                    </li>
                    <li>
                        <p>
                            <m>gH\cap g'H\ne\emptyset</m>.
                        </p>
                    </li>
                </ol>
            </p>
        </li>
        <li>
            <p>
                The cosets of <m>H</m> form a partition of <m>G</m>. That is, we have 
                <md>
                    <mrow>G \amp =\bigcup_{g\in G} gH</mrow>
                </md>
                and
                <me>
                    gH\ne g'H\iff gH\cap g'H=\emptyset
                </me>.
            </p>
        </li>
    </ol>
    </p>
    </statement>
    <proof>
    <p>
        This is another example of a theorem where we get a lot of mileage out of defining an equivalence relation. The relation <m>g\sim g'</m> if and only if <m>g'\in gH</m> is easily seen to be an equivalence relation:
        <md>
            <mrow>g=ge \amp \implies g\in gH</mrow>
            <mrow> \amp \implies g\sim g</mrow>
            <mrow>g \sim g' \amp \implies g'\in gH </mrow>
            <mrow> \amp \implies g'=gh</mrow>
            <mrow> \amp \implies g=g'h^{-1}\in g'H</mrow>
            <mrow> \amp \implies g'\sim g</mrow>
            <mrow>g\sim g' \text{ and } g'\sim g''\amp \implies g'=gh \text{ and } g''=g'h' </mrow>
            <mrow> \amp \implies g''=g'h'=g(hh')\in gH</mrow>
            <mrow> \amp \implies g\sim g''</mrow>
        </md>.
        Since the equivalence classes of <m>\sim</m> are precisely the cosets <m>gH</m> by definition, statement (3) and most of the equivalent statements in (2) follow immediately. The exception is the statement that <m>gH=g'H</m> if and only if <m>g^{-1}g'\in H</m>, which follows using equivalent formulation (b), since 
        <md>
            <mrow>gH=gH' \amp \iff g'\in gH</mrow>
            <mrow> \amp \iff g'=gh \text{ for some } h\in H</mrow>
            <mrow> \amp \iff g^{-1}g'=h \text{ for some } h\in H</mrow>
            <mrow> \amp \iff g^{-1}g'\in H</mrow>
        </md>.
    </p>
    </proof>
    </theorem>
    
    
    <theorem xml:id="th_lagrange">
    <title>Lagrange's theorem</title>
    <statement>
    <p>
    Let <m>H</m> be a subgroup of the group <m>G</m>. 
    <ol>
        <li>
            <p>
                We have 
                <mdn>
                    <mrow>\abs{G} \amp = \abs{H}\abs{G/H}</mrow>
                </mdn>.
                When <m>G</m> is infinite, this can be interpreted as saying <m>H</m> is infinite or <m>G/H</m> is infinite. 
            </p>
        </li>
        <li>
            <p>
                If <m>\abs{G}&lt; \infty</m>, then we have 
                <mdn>
                    <mrow xml:id="eq_lagrange"> \abs{G/H}\amp = \frac{\abs{G}}{\abs{H}} </mrow>
                </mdn>.
            </p>
        </li>
    </ol>
    </p>
    </statement>
    <proof>
    <p>
        Statement (2) follows directly from (1). Statement (1) follows from <xref ref="th_cosets"/> and a counting argument. First observe that for all <m>g\in G</m> we have <m>\abs{H}=\abs{gH}</m> as witnessed by the map
        <md>
            <mrow>H \amp \rightarrow gH</mrow>
            <mrow>h \amp \longmapsto gh</mrow>
        </md>, which has inverse map 
        <md>
            <mrow>gH \amp \mapsto H</mrow>
            <mrow>g' \amp \longmapsto g^{-1}g' </mrow>
        </md>.
         Next, let <m>(g_{\alpha}H)_{\alpha\in I}</m> be the family of <em>distinct</em> cosets, so that we have 
        <md>
            <mrow>\abs{G/H} \amp =\abs{I}</mrow>
            <mrow>G\amp=\bigcup_{\alpha\in I} g_{\alpha}H</mrow>
        </md>
        and <m>g_\alpha H\cap g_\beta H=\emptyset</m> for all <m>\alpha\ne \beta</m>. If <m>I</m> and <m>\abs{H}</m> are both finite, then the sum rule for disjoint sets yields
        <md>
            <mrow>\abs{G} \amp =\sum_{\alpha\in I}\abs{g_{\alpha}H}</mrow>
            <mrow> \amp = \abs{I}\cdot \abs{H} (\abs{g_{\alpha}H}=\abs{H})</mrow>
            <mrow> \amp =\abs{G/H}\abs{H}</mrow>
        </md>. 
        This both proves the result in the case where <m>G</m> is finite, and shows that if <m>G</m> is infinite, than either <m>H</m> or <m>G/H</m> is infinite. 
    </p>
    </proof>
    </theorem>
    <definition xml:id="d_index">
    <title>Index of subgroup</title>
    <notation>
        <usage><m>G\colon H</m></usage>
      <description>index of <m>H</m> in <m>G</m></description>
    </notation>
    <statement>
    <p>
        Given a subgroup <m>H</m> of the group <m>G</m>, its index <m>\abs{G\colon H}</m> is defined as 
        <me>
            \abs{G\colon H}=\abs{G/H}
        </me>.
        In other words, <m>G\colon H</m> is the cardinality of the coset space <m>G/H</m>.
    </p>
    </statement>
    </definition>
    <remark>
        <title>Lagrange's theorem</title>
        
        <p>
            Using the index notation, we can re-write Lagrange's theorem as 
            <me>
                \abs{G}=\abs{H}\abs{G\colon H}
            </me>.
        </p>
    </remark>
    <corollary xml:id="cor_subgroup_card">
        <title>Cardinality of subgroups</title>
        <statement>
            <p>
                Assume <m>G</m> is a finite group. 
                <ol>
                    <li>
                        <p>
                           For any subgroup <m>H\leq G</m>, we have 
                <men xml:id="eq_subgroup_card">
                    \abs{H}\mid \abs{G}
                </men>. 
                        </p>
                    </li>
                    <li>
                        <p>
                            For any <m>g\in G</m> we have 
                            <men xml:id="eq_ord_g_divis">
                                \ord g\mid \abs{G}
                            </men>.
                        </p>
                    </li>
                </ol>
                
                
            </p>
        </statement>
    </corollary>
    <corollary xml:id="cor_groups_prime_card">
        <title>Groups of prime cardinality</title>
        <statement>
            <p>
                If <m>\abs{G}=p</m> for a prime integer <m>p</m>, then <m>G</m> is cyclic. It follows that 
                <me>
                    G\cong \Z/p\Z
                </me>.
            </p>
        </statement>
    </corollary>
    
    
    
    
    

</section>