<?xml version="1.0" encoding="UTF-8"?>

<section xml:id="s_grouprings_polys_quats" xmlns:xi="http://www.w3.org/2001/XInclude">
    <title>Group rings, polynomials, quaternions</title>
    <introduction>
        <p>
            In this section we introduce three ring constructions: group rings, polynomial (and power series) rings, and quaternion rings. Each of these uses as an underling set a collection of <q>formal sums</q> with coefficients in a base ring <m>R</m>. This somewhat ambiguous language of formal sums comes up frequently in mathematics. As we make official with <xref ref="fiat_formal_sums"/> a formal sum is really just a tuple that we have decided to write using summation notation. The definition of the complex numbers is a typical example of this phenomenon: complex numbers are usually defined as a formal sum <m>a+bi</m> where <m>a,b\in \R</m>, when in essence a complex number is just a pair <m>(a,b)\in \R^2</m>. Why not just use tuple notation? We tend to reach for the formal sum notation in situations where there is a (well-behaved) multiplication defined on our tuples, which further more respects the component-wise addition of these tuples. In these situations algebraic manipulation often proceeds more smoothly with the formal sum representation of objects, as opposed to the tuple representation. 
        </p>
        <assumption xml:id="fiat_formal_sums">
            <title>Formal sums are tuples</title>
            <statement>
                <p>
                    Let <m>R</m> be a ring, and let <m>J</m> be a nonempty set. A <em>formal sum</em> of the form 
                    <me>
                        \sum_{j\in J}a_j\, j
                    </me>
                    is just alternative notation for the tuple <m>(a_j)_{j\in J}</m>. As a very important consequence of this identification, formal sums inherit a coefficient-wise notion of equality from tuples. That is,  we have 
                    <md>
                        <mrow>\sum_{j\in J}a_j\, j=\sum_{j\in J}b_j\, j \amp \iff (a_j)_{j\in J}=(b_j)_{j\in J} </mrow>
                        <mrow> \amp \iff a_j=b_j \text{ for all } j\in J</mrow>
                    </md>.
                   As a form of shortening, when expanding out a formal sum <m>\sum_{j\in J}a_j j</m> we will often drop terms where <m>a_j=0</m>. Similarly, we sometimes drop the <m>1</m> in an expression like <m>1\, j</m>, writing just <m>j</m> instead.
                </p>
            </statement>
        </assumption>
    </introduction>
    
    <subsection xml:id="ss_group_rings">
    <title>Group rings</title>
    <activity xml:id="spec_group_rings">
    <title>Group rings</title>
    <statement>
    <p>
    Let <m>R</m> be a nontrivial commutative ring, and let <m>G</m> be a finite group. We define <m>R\, G</m> to be the set of all formal sums 
    <me>
        \sum_{g\in G}a_g g
    </me>,
    where <m>a_g\in R</m> for all <m>g\in G</m>, and we define binary operations <m>+</m> and <m>\cdot</m> as follows: 
    <md>
        <mrow>\sum_{g\in G}a_g g+\sum_{g\in G}b_g g \amp =\sum_{g\in G}(a_g+b_g) g </mrow>
        <mrow> \sum_{g\in G}a_g g\, \cdot\sum_{g\in G}b_g g \amp =
            \sum_{g\in G}c_g g, \amp c_g=\sum_{\substack{h,k\in G\\ hk=g}}a_h b_k </mrow>
    </md>.
    The triple <m>(R\, G, +, \cdot)</m> is a ring called the <term>group ring</term> of <m>G</m> with coefficients in <m>R</m>. The additive and multiplicative identities of <m>R</m> are given as 
    <md>
        <mrow>0 \amp = \sum_{g\in G}0g</mrow>
        <mrow>1 \amp =1e+\sum_{g\ne e}0g</mrow>
    </md>.
    </p>
    </statement>
    </activity>
    <remark>
    <title>Group rings</title>
    <p>
    <ol>
        <li>
            <p>
                The subset <m>\{re\mid r\in R\}</m> is easily seen to be a subring of <m>R\, G</m>. Indeed, using the definition of the group ring operations, we see that
                <md>
                    <mrow>re + se \amp = (r+s) e </mrow>
                    <mrow>re\cdot se \amp =(rs) e</mrow>
                </md>.
                Thus we can think of the subring <m>\{re\mid r\in R\}</m> as a copy of <m>R</m> living as a subset of <m>R\, G</m>. (Later we will be able to say that this subring is <em>isomorphic</em> to <m>R</m>.)  By slight abuse of notation, we will identify <m>R</m> with this subring of <m>R\, G</m>, and sometimes drop the <m>e</m> from the notation <m>r\, e</m>. 
            </p>
        </li>
        <li>
            <p>
                From the group ring operations definition, it follows that 
                <md>
                    <mrow>r\, e \cdot \left(\sum_{g\in G}a_g\, g \right)\amp =\sum_{g\in G}ra_g\, g</mrow>
                    <mrow> \amp =\left(\sum_{g\in G}a_g\, g\right) \cdot r\, e</mrow>
                </md>.
                Identifying <m>R</m> with <m>\{re\mid r\in R\}</m>, we see that <m>R\leq Z(R)</m>. 
            </p>
        </li>
        <li>
            <p>
                We can also think of the group <m>G</m> as sitting inside <m>R\, G</m>, using the identification 
                <md>
                    <mrow>g \amp =1\, g+\sum_{h\ne g}0\, h</mrow>
                </md>.
                With this identification in place, we that the ring multiplication on <m>R\, G</m> extends the group operation of <m>G</m>. That is, given <m>g,h\in G</m>, identifying these as the ring elements <m>1\, g</m> and <m>1\, h</m> and taking their product, we see that 
                <md>
                    <mrow>g\cdot h \amp = gh </mrow>
                </md>.
            </p>
        </li>
        <li>
            <p>
                Combining the previous observations, we can now give a decent motivation for the multiplication operation on <m>R\, G</m>. Namely, it is the unique binary operation on <m>R\, G</m> satisfying the following properties:
                <ol>
                    
                    <li>
                        <p>
                            it distributes over the given addition operation on <m>R\, G</m>; 
                        </p>
                    </li>
                    <li>
                        <p>
                            it extends the group operation in the sense that <m>g\cdot h=gh</m>;
                        </p>
                    </li>
                    <li>
                        <p>
                            we have <m>r\, e\in Z(R\, G)</m> for all <m>r\in R</m> with respect to this multiplication.
                        </p>
                    </li>
                </ol>
                In this sense our multiplication operation is the unique way of extending the group operation of <m>G</m> to a ring operation on <m>R\, G</m> in such a way that our copy of <m>R\leq R\, G</m> lies in the center of <m>R\, G</m>. 
            </p>
        </li>
    </ol>
    </p>
    </remark>
    <example xml:id="eg_group_ring_D3">
    <title>Group ring of <m>D_3</m></title>
    <statement>
    <p>
    Let <m>D_3=\angvec{r,s\mid r^3=s^2=e, srs=r^{-1}}</m>, and consider the group ring <m>\F_3\, D_3</m>.
    <ol>
        <li>
            <p>
                Let <m>a=2r+ s</m> and <m>b=2r^2+r^2s</m>. Compute <m>ab</m> and <m>ba</m>. 
            </p>
        </li>
        <li>
            <p>
                Show that <m>r+r^2</m> is a unit in <m>\F_3\,D_3</m>
            </p>
        </li>
    </ol> 
    </p>
    </statement>
    <solution>
    <p>
    
    </p>
    </solution>
    </example>
    <example xml:id="eg_group_rings">
    <title>Group ring properties</title>
    <statement>
    <p>
    Let <m>R</m> be a nontrivial commutative ring, and let <m>G</m> be a finite group.
    <ol>
        <li>
            <p>
                Prove that <m>R\, G</m> is commutative if and only if <m>G</m> is abelian. 
            </p>
        </li>
        <li>
            <p>
                Consider the element <m>r=\sum_{g\in G}1\, g\in R\, G</m>. Compute <m>g\cdot r</m>, where <m>g</m> is an element of <m>G</m>. Show that <m>R\, G</m> is not a division ring if <m>G</m> is nontrivial. 
            </p>
        </li>
    </ol>
    </p>
    </statement>
    <solution>
    <p>
    
    </p>
    </solution>
    </example>
    
    
    
    </subsection>
    <subsection xml:id="ss_poly_powerseries">
    <title>Polynomials and power series</title>
    <p>
        Whereas normally power series are introduced as a sort of generalization of polynomials, we will take the approach of defining the notion of a ring of power series, and identify a subring as the ring of polynomials. 
    </p>
    <activity xml:id="spec_power_series">
    <title>Power series ring</title>
    <statement>
    <p>
    Let <m>R</m> be a nontrivial commutative ring. We define the set <m>R[[x]]</m> to be the set of all formal sums of the form
    <md>
        <mrow> \sum_{n=0}^\infty a_n x^n \amp </mrow>
    </md>,
    where <m>a_n\in R</m> for all <m>n\in \Z_{\geq 0}</m>, and we define binary operations <m>+</m> and <m>\cdot</m> as follows: 
    <md>
        <mrow>\sum_{n=0}^\infty a_nx^n+\sum_{n=0}^\infty b_nx^n \amp = \sum_{n=0}^\infty (a_n+b_n)x^n</mrow>
        <mrow>\sum_{n=0}^\infty a_nx^n\cdot \sum_{n=0}^\infty b_nx^n \amp = \sum_{n=0}^\infty c_nx^n \amp c_n=\sum_{k=0}^n a_k b_{n-k}</mrow>
    </md>.
    The triple <m>(R[[x]], +,\cdot)</m> is a commutative ring called the <term>power series ring over (or with coefficients in) <m>R</m> in the unknown (or indeterminate) <m>x</m></term>. The additive and multiplicative identities of <m>R[[x]]</m> are given as
    <md number="yes">
        <mrow>0 \amp =\sum_{n=0}^\infty 0x^n = 0+0x+0x^2+\cdots </mrow>
        <mrow>1 \amp =1x^0+\sum_{n=1}^\infty 0x^n =1+0x+0x^2+\cdots </mrow>
    </md>.
  Given a power series <m>\sum_{n=0}^\infty</m>, we call <m>a_nx^n</m> its <term><m>n</m>-th term</term>, and <m>a_n</m> its  <term><m>n</m>-th coefficient</term>.
    </p>
<p> 
    We will use function-like notation to name power series. In more detail, we will refer to power series using function letters like <m>f</m> and <m>g</m>, and will write <m>f(x)=\sum_{n=0}^\infty a_nx_n</m> when explicitly introducing names of coefficients.
</p>
    </statement>
    </activity>
    <remark>
        <title>Power series equality</title>
    <p>
        When are two power series <m>f(x)=\sum_{n=0}^\infty a_nx^n</m> and <m>g(x)=\sum_{n=0}^\infty b_nx^n</m> equal? Identifying these formal sums as tuples <m>(a_n)_{n=0}^\infty</m>, <m>(b_n)_{n=0}^\infty</m>, following <xref ref="fiat_formal_sums"/>, we see that 
        <md number="no">
           <mrow> f=g \iff a_n=b_n \text{ for all } n\in \Z_{\geq 0}</mrow>
        </md>.
    </p>
    </remark>
    
    <p>
        We now identify the ring <m>R[x]</m> of polynomials over <m>R</m> as the subring of <m>R[[x]]</m> consisting of all power series whose coefficients are <q>eventually</q> equal to zero. 
    </p>
    <activity xml:id="spec_poly_ring">
    <title>Polynomial rings</title>
    <statement>
   <p>
  Let <m>R</m> be a nontrivial commutative ring.
  Define the <term>polynomial ring over <m>R</m> in the indeterminate <m>x</m></term> to be the subset <m>R[x]\subseteq R[[x]]</m> of all power series whose coefficients are <em>eventually</em> equal to zero: i.e., 
  <md>
    <mrow>R[x] \amp = \{f(x)=\sum_{n=0}^\infty a_nx^n\in R[[x]]\mid a_n=0 \text{ for all } n&gt;  N \text{ for some } N\in \Z_{\geq 0} \} </mrow>
    <mrow> \amp =\{f\in R[[x]]\mid f(x)=\sum_{n=0}^Na_nx^n \text{ for some } N\in \Z_{\geq 0}, a_n\in R\}</mrow>
  </md>.
  It is easy to see that <m>R[x]</m> is a subring of <m>R[[x]]</m>, and thus a ring in its own right. Restricted to <m>R[x]</m>, the power series multiplication rule becomes the familiar polynomial multiplication rule: 
  <md>
    <mrow>(\anpoly)\amp \cdot (\bmpoly) =\sum_{k=0}^{m+n}c_kx^k</mrow>
     <mrow>c_k\amp =\sum_{j=0}^k a_j b_{k-j}</mrow>
  </md>.
  As illustrated above, when denoting polynomials we will usually drop all the terms with zero coefficients: <eg/>,  <m>f(x)=a_0+a_1x+\cdots +a_nx^n</m>, or <m>f(x)=\anpoly</m>.
</p>

<p>
  Given a nonzero polynomial <m>f\in R[x]</m>, we define its <term>degree</term>, <m>\deg f</m>, to be the smallest <m>n</m> satisfying <m>a_n\ne 0</m>.
  If <m>f(x) = 0</m>, we define <m>\deg f=-\infty</m>.
</p>

<p>
  If <m>f(x)=\anpoly</m> is a polynomial of degree <m>n\ne -\infty</m>, we call <m>a_{n}</m> the <term>leading coefficient</term> of <m>f</m>.
  A polynomial with leading coefficient equal to <m>1\in R</m> is called <term>monic</term>.
</p>
    </statement>
    </activity>
    </subsection>
    <subsection xml:id="ss_quaternions">
    <title>Quaternion rings</title>
    <activity xml:id="spec_quat_rings">
    <title>Quaternion rings</title>
    <statement>
    <p>
    Let <m>R</m> be a nontrivial commutative ring. We define <m>H(R)</m> to be the set of all formal sums 
    <md>
        <mrow>a_1+a_2i+a_3j+a_4k</mrow>
    </md>,
    where <m>a_i\in R</m> for all <m>1\leq i\leq 4</m>. We define addition on <m>H(R)</m> as 
    <md>
        <mrow>(a_1+a_2i+a_3j+a_4k)+(b_1+b_2i+b_3j+b_4k) </mrow>
        <mrow> = (a_1+b_1)+(a_2+b_2)i+(a_3+b_3)j+(a_4+b_4)k</mrow>
    </md>.
    We define multiplication to be the unique associative binary operation <m>\cdot</m> that distributes over the addition operation <m>+</m>, satisfies 
    <md number="yes">
        <mrow>b(a_1+a_2i+a_3j+a_4k) \amp =(a_1+a_2i+a_3j+a_4k)b </mrow>
        <mrow> \amp =ba_1+ba_2i+ba_3j+ba_4k</mrow>
    </md>
    for all 
    <md>
        <mrow>b \amp =b+0i+0j+0k\in H(R)</mrow>
    </md>,
    and satisfies 
    <md number="yes">
        <mrow> i^2\amp =j^2=k^2=-1 </mrow>
        <mrow>ij \amp = k, jk=i,  ki=j</mrow>
    </md>.
    The triple <m>(H(R), +, \cdot)</m> is a ring called the <term>quaternion ring over (or with coefficients in) <m>R</m></term>. 
    </p>
    <p>
        In the special case where <m>R=\R</m>, we denote <m>\HH=H(\R)</m> and call <m>\HH</m> the <term>Hamilton quaternions</term>. 
    </p>
    </statement>
    </activity>
    
    </subsection>
</section>