<?xml version="1.0" encoding="UTF-8"?>

<section xml:id="s_homomorph" xmlns:xi="http://www.w3.org/2001/XInclude">
    <title>Homomorphisms</title>

    <definition xml:id="d_homomorphism">
    <title>Homomorphism</title>
    <statement>
    <p>
    Let <m>G</m> and <m>H</m> be groups. A <term>(group) homomorphism</term> is a map 
    <m>\phi\colon G\rightarrow H</m> satisfying 
    <men xml:id="eq_group_homomorph">
        \phi(g_1g_2)=\phi(g_1)\phi(g_2)
    </men>
    for all <m>g_1,g_2\in G</m>. 
    </p>
    </statement>
    </definition>
    <remark>
        <title>Homomorphism</title>
        <p>
            There is an important subtlety in the defining property <xref ref="eq_group_homomorph"/>: namely, there are two group operations at play. In more detail, the input <m>g_1g_2</m> of <m>\phi</m> on the left side is a product within the domain group <m>G</m>; the right side <m>\phi(g_1)\phi(g_2)</m> on the other hand is a product within the codomain group <m>H</m>. 
        </p>
        <p>
            A useful way of thinking of a group homomorphism is as a function between groups that <em>respects the group structure</em>, in the sense articulated by <xref ref="eq_group_homomorph"/>. You might ask: shouldn't a group homomorphism also <q>respect</q> the group identities and group inverses? It turns out that the property <xref ref="eq_group_homomorph"/> is itself enough to guarantee this.  
        </p>
    </remark>
    <proposition xml:id="prop_homo">
        <title>Homomorphism properties</title>
        <statement>
            <p>
                Let <m>\phi\colon G\rightarrow H</m> be a group homomorphism, and let <m>e_G</m> and <m>e_H</m> be the identity elements of <m>G</m> and <m>H</m>, respectively.
                <ol>
                    <li>
                        <p>
                            <m>\phi(e_G)=\phi(e_H)</m>
                        </p>
                    </li>
                    <li>
                        <p>
                            <m>\phi(g^{-1})=\phi(g)^{-1}</m>
                        </p>
                    </li>
                </ol> 
            </p>
        </statement>
        <proof>
            <p>
                <ol>
                    <li>
                        <p>
                            Since <m>e_G=e_G\, e_G</m> and <m>\phi</m> is a homomorphism,  we have <m>\phi(e_G)=\phi(e_G)\phi(e_G)</m>. Now do some algebra in <m>H</m>:
                            <md>
                                <mrow>  \phi(e_G)\amp =\phi(e_G)\phi(e_G)\amp </mrow>
                                <mrow>\phi(e_G)^{-1}\phi(e_G)\amp =\phi(e_G)^{-1}\phi(e_G)\phi(e_G) \amp </mrow>
                                <mrow>e_H \amp = \phi(e_G)</mrow>
                            </md>.
                        </p>
                    </li>
                    <li>
                        <p>
                            Fix <m>g\in G</m>. We have 
                            <md>
                                <mrow>gg^{-1}=g^{-1}g=e_G \amp \implies \phi(gg^{-1})=\phi(g^{-1}g)=\phi(e_G) </mrow>
                                <mrow> \amp \implies \phi(g)\phi(g^{-1})=\phi(g^{-1})\phi(g)=e_H </mrow>
                                <mrow> \amp \implies \phi(g^{-1})=\phi(g)^{-1} </mrow>
                            </md>,
                            where the last implication follows from the fact that inverses in groups are unique.
                        </p>
                    </li>
                </ol>
            </p>
        </proof>
    </proposition>
    <example xml:id="eg_homos">
    <title>Homormorphisms</title>
    <statement>
    <p>
    Decide whether the given map is a group homormorphism. 
    <ol>
        <li>
            <title>Trivial homomorphism</title>
            <p>
                Let <m>G</m> and <m>H</m> be groups. Define  
                <m>\phi\colon G\rightarrow H</m> as  <m>\phi(g)=e_H</m> for all <m>g\in G</m>.
            </p>
        </li>
        <li>
            <title>Identity map</title>
            <p>
                Let <m>G</m> be a group, and let 
                <m>\id\colon G\rightarrow G</m> be the identity map as usual. 
            </p>
        </li>
        
        <li>
            <p>
                Fix <m>m\in \Z</m> and define <m>\phi\colon \Z\rightarrow \Z</m> as <m>\phi(n)=mn</m>.
            </p>
        </li>
        <li>
            <p>
                Define <m>\phi\colon \Z\rightarrow \Z</m> as <m>\phi(n)=n^2</m>.
            </p>
        </li>
        <li>
            <title>Determinant</title>
            <p>
                Assume <m>R\in \{\Z,\Q,\R,\C\}</m> or <m>R=\Z/m\Z</m> for some positive integer <m>m</m>. Fix a positive integer <m>n</m> and define <m>\phi\colon \GL_n(R)\rightarrow R^*</m> as <m>\phi(A)=\det A</m>. 
            </p>
        </li>
        <li>
            <title>Exponential map</title>
            <p>
                Define <m>\phi\colon \R\rightarrow \R^*</m> as <m>\phi(x)=e^x</m>. 
            </p>
        </li>
    </ol> 
    </p>
    </statement>
    <solution>
    <p>
    
    </p>
    </solution>
    </example>
    <p>
        The following proposition serves as a useful tool for constructing homomorphisms out of <m>D_n</m>. You will prove it in your homework. 
    </p>
    <proposition xml:id="prop_Dn_homo">
        <title>Homomorphisms from <m>D_n</m></title>
        <statement>
            <p>
                Fix an integer <m>n\geq 3</m>, and let <m>D=\angvec{r,s\mid r^n=s^2=e, sr=r^{-1}s}</m>. Given a group <m>G</m> and elements <m>a,b\in G</m> satisfying 
                <md>
                    <mrow>a^n \amp =b^2=e \amp ba\amp =a^{-1}b</mrow>
                </md>,
                the map <m>\phi\colon D_n\rightarrow G</m> defined as 
                <me>
                    \phi(r^is^j)=a^is^j, \ 0\leq i\leq n-1, 0\leq j\leq 1
                </me>
                is a homomorphism. 
            </p>
        </statement>
        <proof>
            <p>
                The proof is left as a homework exercise.
            </p>
        </proof>
    </proposition>
    <definition xml:id="d_isomorphism">
    <title>Isomorphism</title>
    <statement>
    <p>
    An <term>isomorphism</term> is a bijective group homomorphism <m>\phi\colon G\rightarrow H</m>. Groups <m>G</m> and <m>H</m> are <term>isomorphic</term>, denoted <m>G\cong H</m>, if there is an isomorphism <m>\phi\colon G\rightarrow H</m>. 
    </p>
    </statement>
    </definition>
    <example xml:id="eg_Sn">
    <title>Permutation groups</title>
    <statement>
    <p>
    Let <m>A</m> and <m>B</m> be nonempty sets of the same cardinality: <ie/>, <m>\abs{A}=\abs{B}</m>. 

    Prove: <m>S_A\cong S_B</m>. 
    </p>
    </statement>
    <solution>
    <p>
    By definition of cardinality, since <m>\abs{A}=\abs{B}</m>, there exists a bijective function <m>\alpha\colon A\rightarrow B</m>. Using <m>\alpha</m>, we define <m>\phi\colon S_A\rightarrow S_B</m> as 
    <md>
        <mrow>\phi(\sigma) \amp =\alpha\circ \sigma\circ \alpha^{-1}</mrow>
    </md>.
    Let's first see why this is a well-defined map from <m>S_A</m> to <m>S_B</m>. From 
    <md>
        <mrow>\alpha^{-1}\colon B \amp \rightarrow A</mrow>
        <mrow>\sigma\colon A\amp \rightarrow A \amp </mrow>
        <mrow>\alpha\colon A \amp \rightarrow B</mrow>
    </md>,
     we see that 
     <me>
        \alpha\circ\sigma\circ\alpha^{-1}\colon B\rightarrow B
     </me>.
     Next since <m>\alpha, \alpha^{-1},</m> and <m>\sigma</m> are bijective, so is their composition. Thus <m>\phi(\sigma)=\alpha\circ\sigma\circ\alpha^{-1}\in S_B</m>, as desired. 
    </p>
    <p>
        Next, we show <m>\phi</m> is a homomorphism. We must show that <m>\phi(\sigma\tau)=\phi(\sigma)\phi(\tau)</m> for all <m>\sigma, \tau\in S_A</m>. By definition, we have (dropping the <m>\circ</m> symbols)
        <md>
            <mrow>\phi(\sigma)\phi(\tau) \amp =(\alpha\sigma\alpha^{-1})(\alpha\tau\alpha^{-1})</mrow>
            <mrow> \amp = \alpha \sigma \id_A\tau \alpha^{-1}\amp (\alpha^{-1}\circ\alpha=\id_A)</mrow>
            <mrow> \amp = \alpha \sigma \tau \alpha^{-1} \amp (\id_A\circ \tau=\tau) </mrow>
            <mrow> \amp =\phi(\sigma\tau)</mrow>
        </md>.
        This proves <m>\phi</m> is a homomorphism. To show it is bijective, and hence an isomorphism, we will show that it has an inverse function <m>\phi^{-1}\colon S_B\rightarrow S_A</m>. To this end, given <m>\tau\in S_B</m>, define 
        <me>
            \phi^{-1}(\tau)=\alpha^{-1}\circ\tau \circ \alpha
        </me>.
        Reasoning exactly as above, we see that <m>\phi^{-1}</m> is well-defined: <ie/>, <m>\alpha^{-1}\circ\tau\circ\alpha</m> is indeed an element of <m>S_A</m>. Lastly, computations much like the one above show that  
        <md>
            <mrow>\phi^{-1}\circ\phi\, (\sigma) \amp = \sigma \text{ for all } \sigma\in S_A </mrow>
            <mrow>\phi\circ\phi^{-1}\, (\tau) \amp = \tau \text{ for all } \tau\in S_B </mrow>
        </md>
        and thus that the two functions are inverses of one another.
    </p>
    </solution>
    </example>
    
    
    
    
</section>